@prefix brick: <https://brickschema.org/schema/Brick#> .
@prefix ext: <https://example.com/schema/BrickExtension#> .
@prefix owl: <http://www.w3.org/2002/07/owl#> .
@prefix rdfs: <http://www.w3.org/2000/01/rdf-schema#> .
@prefix skos: <http://www.w3.org/2004/02/skos/core#> .

ext:Charge_Remaining a owl:Class ;
    rdfs:label "Charge Remaining" ;
    rdfs:subClassOf ext:UPS_Status ;
    skos:definition "An estimate of the battery charge remaining expressed as a percent of full charge" .

ext:Input_Frequency_Sensor a owl:Class ;
    rdfs:label "Input Frequency Sensor" ;
    rdfs:subClassOf brick:Frequency_Sensor ;
    skos:definition "" .

ext:Input_Voltage_Sensor a owl:Class ;
    rdfs:label "Input Voltage Sensor" ;
    rdfs:subClassOf brick:Voltage_Sensor ;
    skos:definition "Measures the voltage input to some process or device" .

ext:Minutes_Remaining a owl:Class ;
    rdfs:label "Minutes Remaining" ;
    rdfs:subClassOf ext:UPS_Status ;
    skos:definition "An estimate of the time to battery charge depletion under the present load conditions if the utility power is off and remains off, or if it were to be lost and remain off" .

ext:Seconds_On_Battery a owl:Class ;
    rdfs:label "Seconds On Battery" ;
    rdfs:subClassOf ext:UPS_Status ;
    skos:definition "If the UPS is on battery power, the elapsed time since the UPS last switched to battery power" .

ext:UPS a owl:Class ;
    rdfs:label "UPS" ;
    rdfs:subClassOf brick:Electrical_Equipment ;
    skos:definition "Uninteruptible Power Supply" .

ext:UPS_Load a owl:Class ;
    rdfs:label "UPS Load" ;
    rdfs:subClassOf ext:UPS_Status ;
    skos:definition "An estimate of the load connected to the UPS measured in percentage" .

ext:UPS_Status a owl:Class ;
    rdfs:label "UPS Status" ;
    rdfs:subClassOf brick:Status ;
    skos:definition "" .

